
% This LaTeX was auto-generated from MATLAB code.
% To make changes, update the MATLAB code and republish this document.

\documentclass{article}
\usepackage{graphicx}
\usepackage{color}
\usepackage{lmodern}
\usepackage{amsmath}

\sloppy
\definecolor{lightgray}{gray}{0.5}
\setlength{\parindent}{0pt}

\begin{document}

    
    
\subsection*{Contents}

\begin{itemize}
\setlength{\itemsep}{-1ex}
   \item AMSC 460 - EXAM 1
   \item Problem 1 (finished)
   \item Problem 2 (Yup)
   \item Problem 3 (Yup)
   \item Problem 4()
\end{itemize}


\subsection*{AMSC 460 - EXAM 1}

\begin{verbatim}
clear all; format rational; close all; syms f(x) x y
\end{verbatim}


\subsection*{Problem 1 (finished)}
   \[\phi_0(x) =1, \phi_1(x) =x -\alpha_1\]

   \[\alpha_1=\frac{\int_{-1}^{1} w(x)*x\,dx}{\int_{-1}^{1} w(x)\,dx} = \frac{\int_{-1}^{0} x\,dx+ \int_{0}^{1} 3x\,dx}{4} = \frac{1}{4}\]
   \[(\phi_0, \phi_0) = 2, (f,y_0) = \int_{-1}^{1} w(x)x^3\,d = \frac{1}{2}\]
   \[(\phi_1, \phi_1) = \int_{-1}^{1} w(x)(x-1/2)^2\,dx = \int_{-1}^{0} (x-1/2)^2\,dx\ + \int_{0}^{1} 3(x-1/2)^2\,dx = \frac{4}{3}\]
   \[(f_1, \phi_1) = \int_{-1}^{1} w(x)x^3(x-1/2)^2\,dx = \int_{-1}^{0} x^4-(1/2)x^3\,dx + \int_{0}^{1} 3(x^4-(1/2)x^3 \,dx= \frac{11}{20}\]

   \[\phi(x) = \frac{(\phi_1, \phi_0)}{(\phi_0, \phi_0)}*\phi_0(x) + \frac{(f_1, \phi)}{(\phi_1, \phi_1)}*\phi_1(x) = \frac{1/4}{2} + \frac{\frac{11}{20}}{\frac{4}{3}}(x-\frac{1}{2}) = \frac{33x}{80} - \frac{13}{160}\]   
\subsection*{Problem 2 (Yup)}
      
\begin{par}
   $f(x)= 1*\[ \int_{1}^{-1} 1 \,dx \] =2 
\end{par}

   \[w_1*f(-1)+w_2*f'(-1)+w_3*f'(1)+w_4*f(1) = 2\]

   which means:
   
   \[w_1+w_2+w_3+w_4 = 2\]
   \[w_1 +w_4 = 2\]
   \[when f(x) = x, f'(x) =1, -w_1 +w_2+w_3+w_4 =0\]
   \[when f(x) = x^2, f'(x) =2x, w_1 -2*w_2+2*w_3+w_4 =2/3\]
   \[when f(x) = x^3, f'(x) =3x^2, -w_1 +3*w_2+3*w_3+w_4 =0\]
   \[when f(x) = x^4, f'(x) =4x^3, -w_1 -4*w_2+4*w_3+w_4 =2/5\]

   We dont want to consider the forth term since the precision is quadrature. The matrix is

   \[\begin{bmatrix} 1 &0& 0& 1& 2 \\ -1& 1& 1& 1& 0 \\1& -2& 2& 1& 2/3 \\ -1& 3 &3& 1& 0 \end{bmatrix}\]

   solve by matlab shown below:
\begin{verbatim}
   A = [1 0 0 1 2; -1 1 1 1 0; 1 -2 2 1 2/3; -1 3 3 1 0]
   rref(A)
   \end{verbatim}
   
           \color{lightgray} \begin{verbatim}A =
          1              0              0              1              2       
         -1              1              1              1              0       
          1             -2              2              1              2/3     
         -1              3              3              1              0       
   ans =
          1              0              0              0              1       
          0              1              0              0              1/3     
          0              0              1              0             -1/3     
          0              0              0              1              1       
   \end{verbatim} \color{black}

   so we have 
   \[w_1 = 1\]
   \[w_2 = 1/3\]
   \[w_3 = -1/3\]
   \[w_4 = 1\]

\subsection*{Problem 3 (Yup)}
\begin{par}
   (a)
   first we can write two equations base on $y(t)=xt$
   \[3=x\]
   \[2=2x\]
   so write the two equations in matrix form
\end{par} \vspace{1em}
\begin{par}
   \[\begin{pmatrix}3\\ 2 \end{pmatrix}=\begin{pmatrix}1 & 0\\0 & 2
   \end{pmatrix}\begin{pmatrix}x\\ x \end{pmatrix}\]
\end{par} \vspace{1em}

so we can get that the matrix $A=\begin{pmatrix}1, & 0\\
   0, & 2
   \end{pmatrix},b=\begin{pmatrix}3\\
   2
   \end{pmatrix}$
   
   \[r=\begin{pmatrix}1, & 0\\0, & 2
   \end{pmatrix}\begin{pmatrix}x\\x
   \end{pmatrix}-\begin{pmatrix}3\\2
   \end{pmatrix}=\begin{pmatrix}x-3\\2x-2
   \end{pmatrix}\]
   
   Therefore:
   
   \[||r||_{2}^{2}=(x-3)^{2}+(2x-2)^{2}=5x^{2}-14x+3\]
   \[f(x)=||r||_{2}^{2}=5x^{2}-14x+3\]
   
   \[f^{'}(x)=10x-14\]
   
   \[f'(x)=0=10x-14,x=\frac{7}{5}\]
   
   \[||r||_{2}^{2}\]
   \[x=\frac{7}{5}\]
   
   \begin{par}
      ((b)
   \end{par} \vspace{1em}
   
   \[r=\begin{pmatrix}x-3\\2x-2\end{pmatrix}\]
   
   so
   \[||r||_{4}^{4}=(x-3)^{4}+(2x-2)^{4}=17x^{4}-76x^{3}+150x^{2}-172x+97\]



\subsection*{Problem 4}

\begin{par}
Compute the order of the local truncation error for this method.
\end{par} \vspace{1em}

\[f_{i+1}=f(t_{i}+h,y(t_{i}+h))\]

\[y_{i+1}=y(t_{i}+h)=y_{i}+hf_{i}+\frac{h^{2}}{2}y^{''}+\frac{h^{3}}{6}y^{'''}+O(h^{4})\]

\[y_{i-1}=y(t_{i}-h)=y_{i}-hf_{i}+\frac{h^{2}}{2}y^{''}-\frac{h^{3}}{6}y^{'''}+O(h^{4})\]

\[y^{''}=\frac{d^{2}y}{dt^{2}}=\frac{d}{dt}(\frac{dy}{dt})=\frac{df}{dt}=f_{t}+ff_{y}\]

\[f(t_{i}+h,y(t_{i}+h))=f_{i}+h(\frac{\partial}{\partial t}+\frac{\partial y}{\partial t}\frac{\partial}{\partial y})f+\frac{h^{2}}{2}(\frac{\partial}{\partial t}+\frac{\partial y}{\partial t}\frac{\partial}{\partial y})^{2}f+\frac{h^{3}}{6}(\frac{\partial}{\partial t}+\frac{\partial y}{\partial t}\frac{\partial}{\partial y})^{3}f+O(h^{4})\]

so we can get:

\[y^{''}=\frac{df}{dt},y^{'''}=\frac{d^{2}f}{dt^{2}}\]

\[f(t_{i}+h,y(t_{i}+h))=f_{i}+hy^{''}+\frac{h^{2}}{2}y^{'''}+\frac{h^{3}}{6}y^{(4)}+O(h^{4})\]

so we can get that:

\[3y_{i+1}-4y_{i}+y_{i-1}\]

\[=3y_{i}+3hf_{i}+\frac{3h^{2}}{2}y^{''}+\frac{h^{3}}{2}y^{'''}+O(h^{4})-4y_{i}\]

\[+y_{i}-hf_{i}+\frac{h^{2}}{2}y^{''}-\frac{h^{3}}{6}y^{'''}+O(h^{4})\]

\[=2hf_{i}+2h^{2}y^{''}+\frac{h^{3}}{3}y^{'''}+O(h^{4})\]

then:

\[2hf_{i+1}=2hf_{i}+2h^{2}y^{''}+h^{3}y^{'''}+\frac{h^{4}}{3}y^{(4)}+O(h^{5})\]

so we can get

\[3y_{i+1}-4y_{i}+y_{i-1}-2hf_{i+1}\]

\[=2hf_{i}+2h^{2}y^{''}+\frac{h^{3}}{3}y^{'''}+O(h^{4})-(2hf_{i}+2h^{2}y^{''}+h^{3}y^{'''}+\frac{h^{4}}{3}y^{(4)}+O(h^{5}))\]

\[=-\frac{2h^{3}}{3}y^{'''}+O(h^{4})\]

\begin{par}
   The truncation error of the equation below:
\end{par} \vspace{1em}

\[w_{i+1}=\frac{1}{3}(4w_{i}-w_{i-1}+2hf_{i+1})\]

is:

\[LTE=\frac{2}{9}h^{3}y^{'''}+O(h^{4})\]

\end{document}

